common/ListMonadFacts.v
@@ -112,3 +112,55 @@ Proof.
   apply Qtrans with (y := s0);
   [ eapply f_inv; eauto | eapply IHl; eauto ].
 Qed.
+
+Remark map_aux_inv_state :
+  forall {state B C : Type} {l} {f : B -> Mon C} {m} {s : state} {v s'}
+         {Q : state -> state -> Prop},
+    map_aux f l m s = OK v s' ->
+    Reflexive Q ->
+    Transitive Q ->
+    (forall b s1 c s2, f b s1 = OK c s2 -> Q s1 s2) ->
+    Q s s'.
+Proof.
+  induction l; simpl; intros f m s v s' Q e Qrefl Qtrans f_inv; minv e.
+  apply Qrefl.
+  apply Qtrans with (y := s0).
+  eapply f_inv; eauto.
+  eapply IHl; eauto.
+Qed.
+
+Remark map_inv_state :
+  forall {state B C : Type} {l} {f : B -> Mon C} {s : state} {v s'}
+         {Q : state -> state -> Prop},
+    map f l s = OK v s' ->
+    Reflexive Q ->
+    Transitive Q ->
+    (forall b s1 c s2, f b s1 = OK c s2 -> Q s1 s2) ->
+    Q s s'.
+Proof. intros; eapply map_aux_inv_state; eauto. Qed.
+
+Remark tmap_aux_inv_state :
+  forall {state A B C : Type} {l : list A} {f : B -> Mon C} {m Inl2B} {s : state} {v s'}
+         {Q : state -> state -> Prop},
+    tmap_aux f l m Inl2B s = OK v s' ->
+    Reflexive Q ->
+    Transitive Q ->
+    (forall b s1 c s2, f b s1 = OK c s2 -> Q s1 s2) ->
+    Q s s'.
+Proof.
+  induction l; simpl; intros f m Inl2B s v s' Q e Qrefl Qtrans f_inv; minv e.
+  apply Qrefl.
+  apply Qtrans with (y := s0).
+  eapply f_inv; eauto.
+  eapply IHl; eauto.
+Qed.
+
+Remark tmap_inv_state :
+  forall {state A B C : Type} {l : list A} {f : B -> Mon C} {Inl2B} {s : state} {v s'}
+         {Q : state -> state -> Prop},
+    tmap f l Inl2B s = OK v s' ->
+    Reflexive Q ->
+    Transitive Q ->
+    (forall b s1 c s2, f b s1 = OK c s2 -> Q s1 s2) ->
+    Q s s'.
+Proof. intros; eapply tmap_aux_inv_state; eauto. Qed.
