common/ListMonadTactics.v
@@ -23,15 +23,20 @@ Ltac solveSInv H :=
     match type of EQ1 with
     | _ = OK _ ?s2 =>
       (transitivity s2; [ try (solveSInv EQ1) | try (solveSInv EQ2) ])
-      || auto
-    end    
+      || (try (solveSInv EQ1); try (solveSInv EQ2))
+    end
   | (if ?c then _ else _) _ = OK _ _ => destruct c; try (solveSInv H)
-  | iter ?f _ _ = OK _ _ =>
-    eapply iter_inv_state; eauto with typeclass_instances
-  | titer ?f _ _ _ = OK _ _ =>
-    eapply titer_inv_state; eauto with typeclass_instances
-  | foreach ?f _ _ = OK _ _ =>
-    eapply foreach_inv_state; eauto with typeclass_instances
+  | (tmap _ _ _ ?s = OK _ ?s') =>
+    pattern s, s'; eapply (tmap_inv_state H); eauto with typeclass_instances
+  | (map _ _ ?s = OK _ ?s') =>
+    pattern s, s'; eapply (map_inv_state H); eauto with typeclass_instances
+  | (iter ?f _ ?s = OK _ ?s') =>
+    pattern s, s'; eapply (iter_inv_state H); eauto with typeclass_instances
+  | (fold_left ?f _ _ ?s = OK _ ?s') =>
+    pattern s, s'; eapply (foldl_inv_state H); eauto with typeclass_instances
+  | (foreach ?f _ ?s = OK _ ?s') =>
+    pattern s, s'; eapply (foreach_inv_state H); eauto with typeclass_instances
+  | (getv _ _ _ ?s = OK _ ?s') => rewrite (getv_inv_state H); auto
   | (?F _ _ _ _ _ _ _ _ = OK _ _) =>
     ((progress simpl in H) || unfold F in H); try (solveSInv H)
   | (?F _ _ _ _ _ _ _ = OK _ _) =>
@@ -50,25 +55,19 @@ Ltac solveSInv H :=
     ((progress simpl in H) || unfold F in H); try (solveSInv H)
   end.
 
-Definition NatCounter := @Mon nat.
+Ltac solve_listm H :=
+  match type of H with
+  | (tmap _ _ _ ?s = OK _ ?s') =>
+    pattern s, s'; eapply (tmap_inv_state H); eauto with typeclass_instances; clear H
+  | (map _ _ ?s = OK _ ?s') =>
+    pattern s, s'; eapply (map_inv_state H); eauto with typeclass_instances; clear H
+  | (iter ?f _ ?s = OK _ ?s') =>
+    pattern s, s'; eapply (iter_inv_state H); eauto with typeclass_instances; clear H
+  | (fold_left ?f _ _ ?s = OK _ ?s') =>
+    pattern s, s'; eapply (foldl_inv_state H); eauto with typeclass_instances; clear H
+  | (foreach ?f _ ?s = OK _ ?s') =>
+    pattern s, s'; eapply (foreach_inv_state H); eauto with typeclass_instances; clear H
+  | (getv _ _ _ ?s = OK _ ?s') => rewrite (getv_inv_state H); clear H; try reflexivity                                                              
+  end.
 
-Require Import List.
-Import ListNotations.
-
-Definition suml (l : list nat) (x : { n : nat | n > 0 }) : NatCounter unit :=
-  let (m, gt0m) := x in
-  do _ <- iter (fun n s => OK tt (n + s)) l;
-  iter (fun n s => OK tt (n + s)) (l ++ [m]).
-
-Compute (suml [1; 2; 3; 4] (exist _ 1 (Gt.gt_Sn_O 0)) 0).
-
-Lemma suml_inv_S :
-  forall {l x s v s'},
-    suml l x s = OK v s' ->
-    ((fun s1 s2 => s1 > 0 -> s2 > 0) s s').
-Proof.
-  intros until s'; intros e.
-  cbv beta.
-  pattern s, s'.
-Admitted.
   
