sitpn2hvhdl/GenerateArchitectureFacts.v
@@ -1,0 +1,174 @@
+(** * Facts about Architecture Generation *)
+
+Require Import String.
+Require Import common.StateAndErrorMonad.
+Require Import common.StateAndErrorMonadTactics.
+Require Import common.ListMonad.
+Require Import common.ListMonadFacts.
+Require Import common.ListMonadTactics.
+
+Require Import dp.Sitpn.
+
+Require Import sitpn2hvhdl.Sitpn2HVhdl.
+
+(** ** Facts about Place Map Generation *)
+
+Section GenPMap.
+
+  Ltac solve_gen_pmap_entry_sinv :=
+    intros *; intros e; minv e;
+    match goal with
+    | [ H: _ ?st1 = OK _ _ |- ?f ?st1 = ?f ?st2 ] =>
+      solve_listm H;
+      match goal with
+      | [ H: _ ?st1 = OK _ ?st2,  H': _ = OK _ ?st3 |- _ ?st1 = _ ?st3 ] =>
+        transitivity (f st2);
+        [ solveSInv H; intros *; intros e; minv e; auto
+        | solveSInv H'; intros *; intros e; minv e; auto]
+      end
+    end.
+  
+  Lemma gen_pmap_entry_inv_γ :
+    forall {sitpn} {p : P sitpn} {mm s v s'},
+      generate_place_map_entry p mm s = OK v s' ->
+      γ s = γ s'.
+  Proof. try solve_gen_pmap_entry_sinv. Qed.
+
+  Lemma gen_pmap_entry_inv_lofPs :
+    forall {sitpn} {p : P sitpn} {mm s v s'},
+      generate_place_map_entry p mm s = OK v s' ->
+      lofPs s = lofPs s'.
+  Proof. try solve_gen_pmap_entry_sinv. Qed.
+
+End GenPMap.
+
+(** ** Facts about Transition Map Generation *)
+
+Section GenTMap.
+
+  Lemma gen_tmap_entry_inv_γ :
+    forall {sitpn} {t : T sitpn} {s v s'},
+      generate_trans_map_entry t s = OK v s' ->
+      γ s = γ s'.
+  Proof. intros until s'; intros e; minv e; solve_listm EQ1. Qed.
+
+  Lemma gen_tmap_entry_inv_lofPs :
+    forall {sitpn} {t : T sitpn} {s v s'},
+      generate_trans_map_entry t s = OK v s' ->
+      lofPs s = lofPs s'.
+  Proof. intros until s'; intros e; minv e; solve_listm EQ1. Qed.
+  
+End GenTMap.
+
+(** ** Facts about Interconnection Generation *)
+
+Section GenInterconn.
+
+  Lemma connect_fired_port_inv_γ :
+    forall {sitpn} {e} {t : T sitpn} {s v s'},
+      connect_fired_port e t s = OK v s' ->
+      γ s = γ s'.
+  Proof.
+    intros *; intros e1; monadInv e1; solveSInv EQ; minv EQ1;
+      destruct (ListPlus.getv PeanoNat.Nat.eq_dec Transition.fired o); inversion EQ2; auto;
+        destruct s; inversion EQ2; auto;
+          destruct o0; inversion EQ2; auto.
+  Qed.
+  
+  Lemma connect_fired_ports_inv_γ :
+    forall {sitpn} {lofTs : list (T sitpn)} {s v s'},
+      connect_fired_ports lofTs s = OK v s' ->
+      γ s = γ s'.            
+  Proof.
+    intros *; intros e; solveSInv e.
+    intros; eapply connect_fired_port_inv_γ; eauto.
+  Qed.
+
+  Lemma connect_inv_γ :
+    forall {sitpn xcomp ycomp id__x id__y} {s : Sitpn2HVhdlState sitpn} {v s'},
+      connect xcomp ycomp id__x id__y s  = OK v s' ->
+      γ s = γ s'.
+  Proof. intros until s'; intros e; minv e; simpl; reflexivity. Qed.
+
+  Lemma connect_poutputs_inv_γ :
+    forall {sitpn} {pinfo : PlaceInfo sitpn} {hcomp s v s'},
+      connect_place_outputs pinfo hcomp s = OK v s' ->
+      γ s = γ s'.
+  Proof.
+    intros; pattern s, s'; eapply foldl_inv_state; eauto with typeclass_instances.
+    intros until s0'; intros e.
+    simpl in e.
+    unfold connect_popmap_to_tipmap in e.
+    monadInv e; minv EQ.
+    rewrite (getv_inv_state EQ3); rewrite (connect_inv_γ EQ1); clear EQ3 EQ1.
+    destruct x0 as (pcomp1, tcomp1).
+    monadInv EQ2.
+    rewrite (connect_inv_γ EQ); clear EQ.
+    destruct x0 as (pcomp2, tcomp2).
+    monadInv EQ0; rewrite (connect_inv_γ EQ); clear EQ.
+    destruct x0 as (pcomp3, tcomp3); minv EQ1; auto.
+  Qed.
+    
+  Lemma interconnect_p_inv_γ :
+    forall {sitpn} {p : P sitpn} {s v s'},
+      interconnect_p p s = OK v s' ->
+      γ s = γ s'.
+  Proof.
+    intros until s'; intros e; minv e; simpl.
+    solve_listm EQ4; solve_listm EQ5.
+    transitivity (γ s3).
+    erewrite connect_fired_ports_inv_γ; eauto.
+    transitivity (γ s2).
+    erewrite connect_fired_ports_inv_γ; eauto.
+    erewrite connect_poutputs_inv_γ; eauto.  
+  Qed.
+
+End GenInterconn.
+
+(** ** Facts about Architecture Generation Function *)
+
+Lemma gen_arch_inv_γ :
+  forall {sitpn mm s v s'},
+    @generate_architecture sitpn mm s = OK v s' ->
+    γ s = γ s'.
+Proof.
+  intros until s'; intros e; monadFullInv e.
+  match goal with
+  | [ H1: ListMonad.map (generate_trans_map_entry (sitpn:=sitpn)) _ ?st1 = OK _ _,
+          H2: ListMonad.iter _ _ ?st2 = OK _ _
+      |- _ ] =>
+    simpl in H1; simpl in H2;
+    let s1 := fresh "s" in
+    let s2 := fresh "s" in
+    set (s1 := st1) in *; set (s2 := st2) in *; move s2 after s1
+  end.
+  transitivity (γ s4).
+  solveSInv EQ; intros until s3; intros e; eapply gen_pmap_entry_inv_γ; eauto.
+  change (γ s4) with (γ s); transitivity (γ s5).
+  solveSInv EQ1; intros until s3; intros e; eapply gen_tmap_entry_inv_γ; eauto.
+  change (γ s5) with (γ s1); solveSInv EQ3.
+  intros until s3; intros e; eapply interconnect_p_inv_γ; eauto.
+Qed.
+
+Lemma gen_arch_inv_lofPs :
+  forall {sitpn mm s v s'},
+    @generate_architecture sitpn mm s = OK v s' ->
+    lofPs s = lofPs s'.
+Proof.
+  intros until s'; intros e; monadFullInv e.
+  match goal with
+  | [ H1: ListMonad.map (generate_trans_map_entry (sitpn:=sitpn)) _ ?st1 = OK _ _,
+          H2: ListMonad.iter _ _ ?st2 = OK _ _
+      |- _ ] =>
+    simpl in H1; simpl in H2;
+    let s1 := fresh "s" in
+    let s2 := fresh "s" in
+    set (s1 := st1) in *; set (s2 := st2) in *; move s2 after s1
+  end.
+  transitivity (lofPs s4).
+  solveSInv EQ; intros until s3; intros e; eapply gen_pmap_entry_inv_lofPs; eauto.
+  change (lofPs s4) with (lofPs s); transitivity (lofPs s5).
+  solveSInv EQ1; intros until s3; intros e; eapply gen_tmap_entry_inv_lofPs; eauto.
+  change (lofPs s5) with (lofPs s1); solveSInv EQ3.
+  intros until s3; intros e; eapply interconnect_p_inv_lofPs; eauto.
+Qed.
