sitpn2hvhdl/GenerateHVhdlFacts.v
@@ -9,7 +9,9 @@ Require Import common.StateAndErrorMonad.
 Require Import common.StateAndErrorMonadTactics.
 Require Import common.ListMonad.
 Require Import common.ListMonadFacts.
+Require Import common.ListMonadTactics.
 Require Import common.SetoidListFacts.
+Require Import common.ListPlus.
 
 Require Import sitpn.dp.Sitpn.
 Require Import sitpn.dp.SitpnFacts.
@@ -20,6 +22,7 @@ Require Import hvhdl.HVhdlTypes.
 Require Import hvhdl.AbstractSyntax.
 
 Require Import sitpn2hvhdl.Sitpn2HVhdl.
+Require Import sitpn2hvhdl.GenerateInfosFacts.
 
 (** ** Facts about [InputMap_to_AST] Function *)
 
@@ -93,7 +96,7 @@ Section GeneratePlaceCompInst.
   Lemma gen_p_comp_inst_inv_p_comp :
     forall {sitpn x y s v s' id__p gm ipm opm},
       generate_place_comp_inst sitpn y s = OK v s' ->
-      proj1_sig y <> proj1_sig x ->
+      ~Peq x y ->
       InA Pkeq (x, id__p) (p2pcomp (γ s)) ->
       InCs (cs_comp id__p Petri.place_entid gm ipm opm) (beh s) ->
       InA Pkeq (x, id__p) (p2pcomp (γ s')) /\
@@ -121,73 +124,56 @@ Section GeneratePlaceCompInst.
     specialize (HComp_to_comp_inst_inv_state EQ2) as e2; subst s4.
     split; [ apply InA_setv; auto | auto].
   Qed.
-
-  Lemma titer_gen_p_comp_inst_p_comp :
-    forall {sitpn pls} {Inpls2P : forall n : nat, List.In n pls -> P sitpn} {s v s'},
-      titer (generate_place_comp_inst sitpn) pls Inpls2P s = OK v s' ->
-      List.NoDup pls ->
-      (forall x y pfx pfy, x = y <-> proj1_sig (Inpls2P x pfx) = proj1_sig (Inpls2P y pfy)) ->
-      forall n (Innpls : List.In n pls),
-      exists id__p gm ipm opm,
-        InA Pkeq ((Inpls2P n Innpls), id__p) (p2pcomp (γ s')) /\
-        InCs (cs_comp id__p Petri.place_entid gm ipm opm) (beh s').      
+  
+  Lemma iter_gen_p_comp_inst_p_comp :
+    forall {sitpn pls} {s v s'},
+      iter (generate_place_comp_inst sitpn) pls s = OK v s' ->
+      NoDupA Peq pls ->
+      forall p, InA Peq p pls ->
+        exists id__p gm ipm opm,
+          InA Pkeq (p, id__p) (p2pcomp (γ s')) /\
+          InCs (cs_comp id__p Petri.place_entid gm ipm opm) (beh s').
   Proof.
-    intros until Inpls2P; functional induction (titer (generate_place_comp_inst sitpn) pls Inpls2P) using titer_ind.
+    intros until pls; functional induction (iter (generate_place_comp_inst sitpn) pls) using iter_ind.
 
     (* BASE CASE *)
-    - contradiction.
+    - inversion 3.
 
     (* IND. CASE *)
     - intros;
         lazymatch goal with
-        | [ Hm : (do _ <- _; _) _ = _ |- _ ] =>
-          inversion_clear Innpls as [ e_an | HIn_ntl ]; monadInv Hm
+        | [ Hm : (do _ <- _; _) _ = _, Hin: InA _ _ (_ :: _) |- _ ] =>
+          inversion_clear Hin as [ e1 e2 Peq_pb | e1 e2 HIn_ntl ]; monadInv Hm
         end.
 
       (* CASE a = n *)
       + specialize (gen_p_comp_inst_p_comp EQ0) as (id__p, (gm, (ipm, (opm, (Hin_γs', Hin_behs'))))).
         exists id__p, gm, ipm, opm; split; [ | auto].
-        eapply InA_eqk; eauto.
-        unfold Peq; unfold seq; rewrite ((proj1 (H1 a n (in_eq a tl) Innpls)) e_an).
-        reflexivity.
+        eapply InA_eqk; eauto; symmetry; assumption.        
 
       (* CASE n ∈ tl *)
-      + assert (e_pf : forall x y pfx pfy,
-                   x = y <->
-                   proj1_sig (in_T_in_sublist_T a tl pf x pfx) = proj1_sig (in_T_in_sublist_T a tl pf y pfy))
-          by (intros; apply H1; assumption).
-        lazymatch goal with
-        | [ H: List.NoDup _ |- _ ] => inversion_clear H as [ | e1 e2 Hnotin_a_tl Hnodup_tl ]
+      + lazymatch goal with
+        | [ H: NoDupA _ _ |- _ ] => inversion_clear H as [ | e1 e2 Hnotin_a_tl Hnodup_tl ]
         end.
-        specialize (IHm s x s0 EQ Hnodup_tl e_pf n HIn_ntl) as (id__p, (gm, (ipm, (opm, (Hγ, Hincs_comp))))).
-        unfold in_T_in_sublist_T in Hγ.
+        specialize (IHm s x s0 EQ Hnodup_tl p HIn_ntl) as (id__p, (gm, (ipm, (opm, (Hγ, Hincs_comp))))).
 
         (* Apply gen_p_comp_inst_inv_p_comp *)
-        assert (ne_an : a <> n) by (apply (not_in_in_diff (conj Hnotin_a_tl HIn_ntl))).
-        assert (ne_proj1 : proj1_sig (pf a (in_eq a tl)) <> proj1_sig (pf n (in_cons a n tl HIn_ntl)))
-          by (intros e_proj1; rewrite <- ((proj2 (H1 a n (in_eq a tl) (in_cons a n tl HIn_ntl))) e_proj1) in ne_an;
-              contradiction).
-        specialize (gen_p_comp_inst_inv_p_comp EQ0 ne_proj1 Hγ Hincs_comp) as (Hγ', Hincs_comp').
-        exists id__p, gm, ipm, opm; split; [ | auto].
-        specialize ((proj1 (H1 n n (in_cons a n tl HIn_ntl) Innpls)) eq_refl) as e_proj1.
-        eapply InA_eqk; eauto.
+        assert (nPeq : ~Peq p b) by (eapply InA_neqA; eauto).
+        specialize (gen_p_comp_inst_inv_p_comp EQ0 nPeq Hγ Hincs_comp) as (Hγ', Hincs_comp').
+        exists id__p, gm, ipm, opm; auto.
   Qed.
-
+  
   Lemma gen_p_comp_insts_p_comp :
     forall {sitpn s v s'},
       generate_place_comp_insts sitpn s = OK v s' ->
-      List.NoDup (places sitpn) ->
+      Sig_in_List (lofPs s) ->
       forall p, exists id__p gm ipm opm,
           InA Pkeq (p, id__p) (p2pcomp (γ s')) /\
           InCs (cs_comp id__p Petri.place_entid gm ipm opm) (beh s').
   Proof.
-    intros until s'; intros e; unfold generate_place_comp_insts in e; intros Hnodup p.
-    assert (nat_to_P_determ :
-              forall x y (pfx : In_P sitpn x) (pfy : In_P sitpn y),
-                x = y <-> proj1_sig (nat_to_P x pfx) = proj1_sig (nat_to_P y pfy))
-      by (intros; simpl; reflexivity).
-    rewrite <- (eq_sig (nat_to_P (proj1_sig p) (proj2_sig p)) p eq_refl eq_refl).
-    apply (titer_gen_p_comp_inst_p_comp e Hnodup nat_to_P_determ (proj1_sig p) (proj2_sig p)).  
+    intros until s'; intros e; minv e; intros SIL p.
+    eapply iter_gen_p_comp_inst_p_comp; eauto;
+      [ apply (proj2 SIL) | apply ((proj1 SIL) p)].
   Qed.
 
   (** *** NoDup in p2pcomp *)
@@ -221,51 +207,43 @@ Section GeneratePlaceCompInst.
         rewrite <- e2, <- e1; clear e1 e2; simpl; auto with setoidl.
   Qed.
 
-  Lemma titer_gen_p_comp_inst_inv_nodup_p2pcomp :
-    forall {sitpn pls} {Inpls2P : forall n : nat, List.In n pls -> P sitpn} {s v s'},
-      titer (generate_place_comp_inst sitpn) pls Inpls2P s = OK v s' ->
-      (forall x pfx, x = proj1_sig (Inpls2P x pfx)) ->
+  Lemma iter_gen_pcomp_inst_inv_nodup_p2pcomp :
+    forall {sitpn pls} {s v s'},
+      iter (generate_place_comp_inst sitpn) pls s = OK v s' ->
       forall p,
         ~InA Peq p (fs (p2pcomp (γ s))) ->
-        ~List.In (proj1_sig p) pls ->
+        ~InA Peq p pls ->
         ~InA Peq p (fs (p2pcomp (γ s'))).
   Proof.
-    intros until Inpls2P;
-      functional induction (titer (generate_place_comp_inst sitpn) pls Inpls2P) using titer_ind;
+    intros until pls;
+      functional induction (iter (generate_place_comp_inst sitpn) pls) using iter_ind;
       intros s v s' e; monadInv e; auto; intros.
-    eapply gen_p_comp_inst_inv_p2pcomp; eauto.
-    unfold Peq; unfold seq.
-    lazymatch goal with
-    | [ e1: forall _ _, _ = proj1_sig _, H: ~List.In _ (_ :: _) |- _ ] =>
-      rewrite <- (e1 a (in_eq a tl));
-        rewrite not_in_cons in H1; apply proj1 in H1; auto
-    end.
+    eapply gen_p_comp_inst_inv_p2pcomp; eauto with setoidl.
+    intro; apply H0; symmetry in H1; auto.
   Qed.
 
-  Lemma titer_gen_p_comp_inst_nodup_p2pcomp :
-    forall {sitpn pls} {Inpls2P : forall n : nat, List.In n pls -> P sitpn} {s v s'},
-      titer (generate_place_comp_inst sitpn) pls Inpls2P s = OK v s' ->
-      List.NoDup pls ->
-      (forall n (Innpls : List.In n pls), ~InA Peq (Inpls2P n Innpls) (fs (p2pcomp (γ s)))) ->
-      (forall x pfx, x = proj1_sig (Inpls2P x pfx)) ->
+  Lemma iter_gen_pcomp_inst_nodup_p2pcomp :
+    forall {sitpn pls s v s'},
+      iter (generate_place_comp_inst sitpn) pls s = OK v s' ->
+      NoDupA Peq pls ->
+      (forall p, InA Peq p pls -> ~InA Peq p (fs (p2pcomp (γ s)))) ->
       NoDupA Peq (fs (p2pcomp (γ s))) ->
       NoDupA Peq (fs (p2pcomp (γ s'))).
   Proof.
-    intros until Inpls2P;
-      functional induction (titer (generate_place_comp_inst sitpn) pls Inpls2P) using titer_ind;
+    intros until pls;
+      functional induction (iter (generate_place_comp_inst sitpn) pls) using iter_ind;
       intros s v s' e; monadInv e; auto; intros.
     
     eapply gen_p_comp_inst_nodup_p2pcomp; eauto;
       lazymatch goal with
-      | [ H: forall _ _, _ = proj1_sig _, Hnd: List.NoDup (_ :: _) |- _ ] =>
-        (eapply titer_gen_p_comp_inst_inv_nodup_p2pcomp; eauto;
-         rewrite <- (H a (in_eq a tl));
-         apply (proj1 (proj1 (NoDup_cons_iff a tl) Hnd)))
-        || (eapply IHm; eauto; apply (proj2 (proj1 (NoDup_cons_iff a tl) Hnd)))
+      | [ Hnd: NoDupA _ (?a :: ?tl), Hnin: forall _, _ -> ~_ |- _ ] =>
+        (eapply iter_gen_pcomp_inst_inv_nodup_p2pcomp; eauto; [
+           apply Hnin; apply InA_cons_hd; reflexivity
+         | inversion Hnd; assumption])
+        || (eapply IHm; eauto; inversion Hnd; assumption)
       end.
   Qed.
-
-  
+    
 End GeneratePlaceCompInst.
 
 (** ** Facts about Generation of T Component Instances *)
@@ -282,20 +260,16 @@ Section GenerateTransCompInst.
       specialize (HComp_to_comp_inst_inv_state EQ0) as e2;
       rewrite <- e2, <- e1; clear e1 e2; simpl; reflexivity.
   Qed.
-
-  Lemma titer_gen_t_comp_inst_inv_p2pcomp :
-    forall {sitpn trs} {Intrs2T : forall n : nat, List.In n trs -> T sitpn} {s v s'},
-      titer (generate_trans_comp_inst sitpn) trs Intrs2T s = OK v s' ->
+  
+  Lemma iter_gen_tcomp_inst_inv_p2pcomp :
+    forall {sitpn trs s v s'},
+      iter (generate_trans_comp_inst sitpn) trs s = OK v s' ->
       p2pcomp (γ s) = p2pcomp (γ s').
   Proof.
-    intros until Intrs2T;
-      functional induction (titer (generate_trans_comp_inst sitpn) trs Intrs2T) using titer_ind;
-      intros s v s' e; monadInv e;
-        [ auto |
-          transitivity (p2pcomp (γ s0));
-          [eapply IHm; eauto | eapply gen_t_comp_inst_inv_p2pcomp; eauto] ].
+    intros until s'; intros e; solveSInv e.
+    intros; eapply gen_t_comp_inst_inv_p2pcomp; eauto.
   Qed.
-
+  
   Lemma gen_t_comp_inst_inv_in_beh :
     forall {sitpn t s v s'},
       generate_trans_comp_inst sitpn t s = OK v s' ->
@@ -309,20 +283,15 @@ Section GenerateTransCompInst.
     intros; right; assumption.
   Qed.
 
-  Lemma titer_gen_t_comp_inst_inv_in_beh :
-    forall {sitpn trs} {Intrs2T : forall n : nat, List.In n trs -> T sitpn} {s v s'},
-      titer (generate_trans_comp_inst sitpn) trs Intrs2T s = OK v s' ->
+  Lemma iter_gen_tcomp_inst_inv_in_beh :
+    forall {sitpn trs s v s'},
+      iter (generate_trans_comp_inst sitpn) trs s = OK v s' ->
       forall cstmt, InCs cstmt (beh s) -> InCs cstmt (beh s').
   Proof.
-    intros until Intrs2T;
-      functional induction (titer (generate_trans_comp_inst sitpn) trs Intrs2T) using titer_ind;
-      intros s v s' e; monadInv e;
-        [auto
-        | intros cstmt Hincs;
-          specialize (IHm s x s0 EQ cstmt Hincs);
-          eapply gen_t_comp_inst_inv_in_beh; eauto].
+    intros until s'; intros e; solveSInv e.
+    intros; eapply gen_t_comp_inst_inv_in_beh; eauto.
   Qed.
-
+  
   Lemma gen_t_comp_insts_inv_p_comp :
     forall {sitpn s v s' p id__p gm ipm opm},
       generate_trans_comp_insts sitpn s = OK v s' ->
@@ -331,10 +300,10 @@ Section GenerateTransCompInst.
       InA Pkeq (p, id__p) (p2pcomp (γ s')) /\
       InCs (cs_comp id__p Petri.place_entid gm ipm opm) (beh s').
   Proof.
-    intros until opm; intros e; unfold generate_trans_comp_insts in e.
+    intros until opm; intros e; monadFullInv e.
     split;
-      [rewrite <- (titer_gen_t_comp_inst_inv_p2pcomp e); assumption |
-       eapply titer_gen_t_comp_inst_inv_in_beh; eauto].
+      [rewrite <- (iter_gen_tcomp_inst_inv_p2pcomp EQ0); assumption |
+       eapply iter_gen_tcomp_inst_inv_in_beh; eauto].
   Qed.
 
 End GenerateTransCompInst.
@@ -346,18 +315,34 @@ Section Sitpn2HVhdl.
   Lemma gen_comp_insts_p_comp :
     forall {sitpn s v s'},
       generate_comp_insts sitpn s = OK v s' ->
-      List.NoDup (places sitpn) ->
+      Sig_in_List (lofPs s) ->
       forall p, exists id__p gm ipm opm,
           InA Pkeq (p, id__p) (p2pcomp (γ s')) /\
           InCs (cs_comp id__p Petri.place_entid gm ipm opm) (beh s').
   Proof.
-    intros until s'; intros e; monadInv e; intros Hnodup p.
-    specialize (gen_p_comp_insts_p_comp EQ Hnodup p)
+    intros until s'; intros e; monadInv e; intros Hsil p.
+    specialize (gen_p_comp_insts_p_comp EQ Hsil p)
       as (id__p, (gm, (ipm, (opm, (Hin_γs0, Hin_behs0))))).
     exists id__p, gm, ipm, opm.
     eapply gen_t_comp_insts_inv_p_comp; eauto.
   Qed.
 
+  Lemma gen_arch_inv_lofPs :
+    forall {sitpn mm} {s : Sitpn2HVhdlState sitpn} {v s'},
+      generate_architecture mm s = OK v s' ->
+      Sig_in_List (lofPs s) ->
+      Sig_in_List (lofPs s').
+  Proof.
+    
+  Admitted.
+
+  Lemma gen_ports_inv_lofPs :
+    forall {sitpn} {s : Sitpn2HVhdlState sitpn} {v s'},
+      generate_ports s = OK v s' ->
+      Sig_in_List (lofPs s) ->
+      Sig_in_List (lofPs s').
+  Admitted.
+  
   Lemma sitpn2hvhdl_p_comp :
     forall {sitpn decpr id__ent id__arch mm d γ},
       (* [sitpn] translates into [(d, γ)]. *)
@@ -367,7 +352,7 @@ Section Sitpn2HVhdl.
           InA Pkeq (p, id__p) (p2pcomp γ) /\
           InCs (cs_comp id__p Petri.place_entid gm ipm opm) (behavior d).
   Proof.
-    intros.  
+    intros. 
     functional induction (sitpn_to_hvhdl sitpn decpr id__ent id__arch mm) using sitpn_to_hvhdl_ind.
     
     (* Error *)
@@ -380,7 +365,10 @@ Section Sitpn2HVhdl.
     lazymatch goal with
     | [ H: inl _ = inl _, Hwd: IsWellDefined _ |- _ ] =>
       let NoDupPlaces := (get_nodup_places Hwd) in
-      specialize (gen_comp_insts_p_comp EQ2 NoDupPlaces p)
+      let sil_lofPs_s := constr:(gen_sitpn_infos_sil_lofPs EQ NoDupPlaces) in
+      let sil_lofPs_s0 := constr:(gen_arch_inv_lofPs EQ1 sil_lofPs_s) in
+      let sil_lofPs_s1 := constr:(gen_ports_inv_lofPs EQ0 sil_lofPs_s0) in
+      specialize (gen_comp_insts_p_comp EQ2 sil_lofPs_s1 p)
         as (id__p, (gm, (ipm, (opm, (Hin_γs2, Hin_behs2)))));
         exists id__p, gm, ipm, opm;
         monadFullInv EQ4; inversion H; subst; simpl; auto
@@ -396,7 +384,7 @@ Section Sitpn2HVhdl.
       NoDupA Peq (fs (p2pcomp (γ s'))).
   Proof.
     intros until s'; intros e; monadInv e; intros.
-    rewrite <- (titer_gen_t_comp_inst_inv_p2pcomp EQ0).
+    rewrite <- (iter_gen_t_comp_inst_inv_p2pcomp EQ0).
     eapply titer_gen_p_comp_inst_nodup_p2pcomp; eauto.
   Qed.
 
