sitpn2hvhdl/GenerateInfosFacts.v
@@ -1,0 +1,268 @@
+(** * Facts about Sitpn Information Generation Functions *)
+
+Require Import common.Coqlib.
+Require Import common.StateAndErrorMonad.
+Require Import common.StateAndErrorMonadTactics.
+Require Import common.ListDep.
+Require Import common.ListMonad.
+Require Import common.ListMonadFacts.
+Require Import common.ListMonadTactics.
+Require Import common.ListPlus.
+Require Import common.GlobalFacts.
+
+
+Require Import sitpn.dp.Sitpn.
+Require Import sitpn.dp.SitpnFacts.
+
+Require Import sitpn2hvhdl.Sitpn2HVhdl.
+
+(** ** Facts about Transition Information Generation *)
+
+Section TInfos.
+
+  Lemma gen_tinfos_inv_γ :
+    forall {sitpn s v s'},
+      generate_trans_infos sitpn s = OK v s' ->
+      γ s = γ s'.
+  Proof.
+    intros until s'; intros e; solveSInv e. 
+    intros until s2; intros e1; pattern s1, s2; minv e1; simpl; reflexivity.
+  Qed.
+
+  Lemma gen_tinfos_inv_lofPs :
+    forall {sitpn s v s'},
+      generate_trans_infos sitpn s = OK v s' ->
+      lofPs s = lofPs s'.
+  Proof.
+    intros until s'; intros e; solveSInv e. 
+    intros until s2; intros e1; pattern s1, s2; minv e1; simpl; reflexivity.
+  Qed.
+    
+End TInfos.
+
+(** ** Facts about Place Information Generation *)
+
+Section PInfos.
+
+  Lemma all_conflicts_solved_by_mutex_inv_state :
+    forall {sitpn lofTs s v s'},
+      all_conflicts_solved_by_mutex sitpn lofTs s = OK v s' ->
+      s = s'.
+  Proof.
+    induction lofTs; simpl; intros until s'; intros e; minv e; auto.
+    transitivity s0.
+    - eapply find_inv_state; eauto with typeclass_instances.
+      intros until s2; intros e1; pattern s1, s2; minv e1;
+        (transitivity s6; [ eauto with listmonad | ];
+         transitivity s4; [ eauto with listmonad | ];
+         transitivity s5; [ eauto with listmonad | ];
+         eauto with listmonad).
+    - eapply IHlofTs; eauto.
+    - eapply find_inv_state; eauto with typeclass_instances.
+      intros until s2; intros e1; pattern s1, s2; minv e1;
+        (transitivity s5; [ eauto with listmonad | ];
+         transitivity s3; [ eauto with listmonad | ];
+         transitivity s4; [ eauto with listmonad | ];
+         eauto with listmonad).
+  Qed.
+
+  Lemma sort_by_priority_inv_state :
+    forall {sitpn decpr lofTs s v s'},
+      sort_by_priority sitpn decpr lofTs s = OK v s' ->
+      s = s'.
+  Proof.
+    intros until s'; intros e; unfold sort_by_priority in e.
+    eapply foldl_inv_state; eauto with typeclass_instances.
+    intros until s0; cbv beta.
+    functional induction (inject_t sitpn decpr a b) using inject_t_ind;
+      intros until s0'; intros f; minv f; auto.
+    eapply IHc; eauto. 
+  Qed.
+
+  Lemma gen_pinfos_inv_γ :
+    forall {sitpn decpr s v s'},
+      generate_place_infos sitpn decpr s = OK v s' ->
+      γ s = γ s'.
+  Proof.
+    intros until s'; intros e; solveSInv e.
+    intros until s2; intros e1; pattern s1, s2; monadInv e1; simpl.
+    transitivity (γ s).
+    minv EQ; auto.
+    minv EQ1; ((rewrite (all_conflicts_solved_by_mutex_inv_state EQ2); simpl; reflexivity)
+               || (rewrite (all_conflicts_solved_by_mutex_inv_state EQ2), (sort_by_priority_inv_state EQ1); simpl; reflexivity)).
+  Qed.
+
+  Lemma gen_pinfos_inv_lofPs :
+    forall {sitpn decpr s v s'},
+      generate_place_infos sitpn decpr s = OK v s' ->
+      lofPs s = lofPs s'.
+  Proof.
+    intros until s'; intros e; solveSInv e.
+    intros until s2; intros e1; pattern s1, s2; monadInv e1; simpl.
+    transitivity (lofPs s).
+    minv EQ; auto.
+    minv EQ1; ((rewrite (all_conflicts_solved_by_mutex_inv_state EQ2); simpl; reflexivity)
+               || (rewrite (all_conflicts_solved_by_mutex_inv_state EQ2), (sort_by_priority_inv_state EQ1); simpl; reflexivity)).
+  Qed.
+  
+End PInfos.
+
+(** ** Facts about Generation of Interpretation Information *)
+
+Section InterprInfos.
+
+  Lemma gen_cinfos_inv_γ :
+    forall {sitpn s v s'},
+      generate_cond_infos sitpn s = OK v s' ->
+      γ s = γ s'.
+  Proof.
+    intros until s'; intros e; pattern s, s'; solveSInv e.
+    intros until s2; intros e1; pattern s1, s2; minv e1; simpl; reflexivity.
+  Qed.
+
+  Lemma gen_cinfos_inv_lofPs :
+    forall {sitpn s v s'},
+      generate_cond_infos sitpn s = OK v s' ->
+      lofPs s = lofPs s'.
+  Proof.
+    intros until s'; intros e; pattern s, s'; solveSInv e.
+    intros until s2; intros e1; pattern s1, s2; minv e1; simpl; reflexivity.
+  Qed.
+  
+  Lemma gen_ainfos_inv_γ :
+    forall {sitpn s v s'},
+      generate_action_infos sitpn s = OK v s' ->
+      γ s = γ s'.
+  Proof.
+    intros until s'; intros e; pattern s, s'; solveSInv e.
+    intros until s2; intros e1; pattern s1, s2; minv e1; simpl; reflexivity.
+  Qed.
+
+  Lemma gen_ainfos_inv_lofPs :
+    forall {sitpn s v s'},
+      generate_action_infos sitpn s = OK v s' ->
+      lofPs s = lofPs s'.
+  Proof.
+    intros until s'; intros e; pattern s, s'; solveSInv e.
+    intros until s2; intros e1; pattern s1, s2; minv e1; simpl; reflexivity.
+  Qed.
+  
+  Lemma gen_finfos_inv_γ :
+    forall {sitpn s v s'},
+      generate_fun_infos sitpn s = OK v s' ->
+      γ s = γ s'.
+  Proof.
+    intros until s'; intros e; pattern s, s'; solveSInv e.
+    intros until s2; intros e1; pattern s1, s2; minv e1; simpl; reflexivity.
+  Qed.
+
+  Lemma gen_finfos_inv_lofPs :
+    forall {sitpn s v s'},
+      generate_fun_infos sitpn s = OK v s' ->
+      lofPs s = lofPs s'.
+  Proof.
+    intros until s'; intros e; pattern s, s'; solveSInv e.
+    intros until s2; intros e1; pattern s1, s2; minv e1; simpl; reflexivity.
+  Qed.
+
+End InterprInfos.
+
+(** ** Facts about Checking of Sitpn Well-definition *)
+
+Section CheckWDSitpn.
+
+  Lemma check_wd_sitpn_inv_eq_state :
+    forall {sitpn decpr s v s'},
+      check_wd_sitpn sitpn decpr s = OK v s' ->
+      s = s'.
+  Proof.  
+    intros until s'; intros e; solveSInv e; auto.
+    intros until s3; intros e1; minv e1; auto.
+    intros until s3; intros e1; solveSInv e1; auto.
+    intros until s5; intros e2; solveSInv e2; auto.
+    intros until s7; intros e3; solveSInv e3; auto.
+  Qed.
+  
+End CheckWDSitpn.
+
+(** ** Facts about Dependently-typed Lists Generation *)
+
+Lemma tmap_aux_sil_lofPs :
+  forall {sitpn Nats Pls} {InNats2P : forall n : nat, List.In n Nats -> P sitpn}
+         {s : Sitpn2HVhdlState sitpn} {lofPs s'},
+    tmap_aux (fun p s => Ret p s) Nats Pls InNats2P s = OK lofPs s' ->
+    (forall p, List.In (proj1_sig p) Nats \/ InA Peq p Pls) ->
+    (forall x (InxNats : List.In x Nats), x = proj1_sig (InNats2P x InxNats)) ->
+    (forall x (InxNats : List.In x Nats), ~InA Peq (InNats2P x InxNats) Pls) ->
+    List.NoDup Nats ->
+    NoDupA Peq Pls ->
+    Sig_in_List lofPs.
+Proof.
+  induction Nats; intros until s'; intros e; minv e; intros.
+
+  - split; [ firstorder | auto ].
+  - eapply IHNats; eauto.
+    + intros p; specialize (H p); inversion_clear H as [In_aNats | InA_Pls].
+      -- inversion_clear In_aNats as [e_proj1p_a | In_Nats].
+         ++ right; eapply (InA_app_iff seq Pls _ _); right.
+            eapply InA_cons_hd; specialize (H0 a (in_eq a Nats)).
+            transitivity a; [auto | auto].
+         ++ auto.
+      -- right; eapply (InA_app_iff seq Pls _ _); left; auto.
+    + intros *; intros InA_Pls_app. erewrite InA_app_iff in InA_Pls_app.
+      inversion_clear InA_Pls_app as [InA_Pls | InA_singleton].
+      -- unfold in_T_in_sublist_T in InA_Pls.
+         specialize (H1 x (in_cons a x Nats InxNats)); contradiction.
+      -- inversion_clear InA_singleton as [e1 e2 Peq_InNats2P | e1 e2 InAnil]; [ | inversion InAnil].
+         unfold in_T_in_sublist_T in Peq_InNats2P.
+         assert (e_ax : a = x) by
+             (transitivity (proj1_sig (InNats2P a (in_eq a Nats)));
+              [eapply H0 | rewrite <- Peq_InNats2P; symmetry; eapply H0]).
+         rewrite e_ax in H2; inversion H2; contradiction.
+    + inversion H2; assumption.
+    + eapply NoDupA_app; eauto.
+      apply NoDupA_singleton.
+      intros; inversion_clear H5 as [e1 e2 Peq_x_InNats2P | e1 e2 InAnil]; [ | inversion InAnil].
+      apply (H1 a (in_eq a Nats)); eapply InA_eqA; eauto with typeclass_instances.
+Qed. 
+
+(** ** Facts about Sitpn Information Generation Function *)
+
+Lemma gen_sitpn_infos_inv_γ :
+  forall {sitpn decpr s v s'},
+    generate_sitpn_infos sitpn decpr s = OK v s' ->
+    γ s = γ s'.
+Proof.
+  intros until s'; intros e; monadInv e.
+  do 10 (match goal with
+        | [ H: ?F _ ?st0 = OK _ ?st1 |- γ ?st0 = γ ?st2 ] =>
+          transitivity (γ st1); [
+            (let e := fresh "e" in solveSInv H; intros *; intros e; minv e; auto)
+            || (minv H; simpl; auto) |];
+          clear H
+        end).
+  rewrite (check_wd_sitpn_inv_eq_state EQ9), (gen_tinfos_inv_γ EQ10), (gen_pinfos_inv_γ EQ11),
+  (gen_cinfos_inv_γ EQ12), (gen_ainfos_inv_γ EQ13).
+  apply (gen_finfos_inv_γ EQ15).
+Qed.
+
+Lemma gen_sitpn_infos_sil_lofPs :
+  forall {sitpn decpr s v s'},
+    generate_sitpn_infos sitpn decpr s = OK v s' ->
+    List.NoDup (places sitpn) ->
+    Sig_in_List (lofPs s').
+Proof.
+  intros until s'; intros e; monadInv e; intros.
+  rewrite <- (gen_finfos_inv_lofPs EQ15); clear EQ15.
+  rewrite <- (gen_ainfos_inv_lofPs EQ13); clear EQ13.
+  rewrite <- (gen_cinfos_inv_lofPs EQ12); clear EQ12.
+  rewrite <- (gen_pinfos_inv_lofPs EQ11); clear EQ11.
+  rewrite <- (gen_tinfos_inv_lofPs EQ10); clear EQ10.
+  rewrite <- (check_wd_sitpn_inv_eq_state EQ9); clear EQ9.
+  do 5 (match goal with
+        | [ H: ?F _ _ = OK _ ?st1 |- Sig_in_List (lofPs ?st1) ] =>
+          minv H; simpl; auto; clear H
+        end).
+  eapply tmap_aux_sil_lofPs; eauto;
+    [intros; left; exact (proj2_sig p) | inversion 1].
+Qed.
